src/Language.v
@@ -53,4 +53,5 @@ Parameter Entry: ClN.
 Parameter EntryClass: Class.
 
 Definition ct (C:ClN) := match C with | cln n => nth n Ξ EntryClass end.
+Parameter EntryClass_ct : ct Entry = EntryClass.
 Definition main: Mtd := 0.
